Add FingerTreeInterface

src/FingerTree.v
@@ -95,6 +95,15 @@ Definition more0 {a:Type} (q: Seq (Tuple a)) (u: Crowd a) : Seq a :=
    | (More (Three (Triple x _ _) _ _) _ _, _) => More (One x) (map1 chop q)u 
    end.
 
+Definition tail {a:Type} (t: Seq a) : Seq a :=
+  match t with
+  | Nil => Nil
+  | Unit x => Nil
+  | More (One _) q u => more0 q u
+  | More (Two x y) q u => More (One y) q u
+  | More (Three x y z) q u => More (Two y z) q u
+  end.
+
 Fixpoint toTuples {a:Type} (la : list a) : list (Tuple a) := 
   match la with
     | [] => []
@@ -127,3 +136,10 @@ Fixpoint fromTuples {a:Type} (lta : list (Tuple a)) : list a :=
   | (Triple x y z :: xs) => [x; y; z] ++ fromTuples xs
   end.
 
+(** Utils *)
+
+Fixpoint depth {a} (t: Seq a) : nat :=
+  match t with
+  | More _ t _ => 1 + depth t
+  | _ => 0
+  end.
