src/QueueInterface.v
@@ -17,7 +17,7 @@ Inductive Op : Type :=
 | Pop
 .
 
-Definition queue_eval_op (o : Op) (vs : list (Queue a)) : list (Queue a) :=
+Definition eval_op_queue (o : Op) (vs : list (Queue a)) : list (Queue a) :=
   match o, vs with
   | Empty, _ => [empty]
   | Push x, q :: _ => [push q x]
@@ -29,69 +29,63 @@ Definition queue_eval_op (o : Op) (vs : list (Queue a)) : list (Queue a) :=
   | _, _ => []
   end.
 
-#[global] Instance PureImpl_Queue : PureImpl Op (Queue a) := queue_eval_op.
+#[global] Instance PureImpl_Queue : PureImpl Op (Queue a) := eval_op_queue.
 
 #[global] Instance CostSpec_Queue : CostSpec Op (Queue a) :=
   fun o vs =>
     match o with
-    | Empty => 1
-    | Push _ => 1
-    | Pop => 1
+    | Empty | Push _ | Pop => 1
     end.
 
-Definition cost (_ : Op) (_ : list (Queue a)) : nat := 7.
+Definition QAa := QueueA a.
 
-Definition TQueueA := T (QueueA a).
-
-Definition queue_exec_op (o : Op) (vs : list TQueueA) : M (list TQueueA) :=
+Definition exec_op_queue (o : Op) (vs : list QAa) : M (list QAa) :=
   match o, vs with
-  | Empty, _ => let~ q := emptyA in ret [q]
-  | Push x, q :: _ => let~ q' := pushA q (Thunk x) in ret [q']
+  | Empty, _ => let! q := emptyA in ret [q]
+  | Push x, q :: _ => let! q' := pushA (Thunk q) (Thunk x) in ret [q']
   | Pop, q :: _ =>
-    let! pop_q := popA q in
+    let! pop_q := popA (Thunk q) in
     match pop_q with
     | None => ret []
-    | Some (x, q) => ret [q]
+    | Some (x, q) => let! q := force q in ret [q]
     end
   | _, _ => ret []
   end.
 
-#[global] Instance CvImpl_Queue : CvImpl Op TQueueA := queue_exec_op.
+#[global] Instance CvImpl_Queue : CvImpl Op QAa := exec_op_queue.
 
 #[local] Instance exec_op_mon (o : Op) :
   Morphisms.Proper (Morphisms.respectful less_defined less_defined)
-    (exec_op (op := Op) (valueA := TQueueA) o).
+    (exec_op (op := Op) (valueA := QAa) o).
 Proof.
   intros ? ? E. destruct o; cbn.
   - reflexivity.
   - destruct E as [ | ? ? ? ? E1 E].
     + reflexivity.
-    + apply bind_mon; [ apply thunk_mon, pushA_mon; reflexivity + auto | intros; apply ret_mon ].
-      constructor; constructor + auto.
+    + apply bind_mon; [ apply pushA_mon; reflexivity + auto | intros; apply ret_mon ].
+      constructor; [ auto | constructor ].
   - destruct E as [ | ? ? ? ? E1 E ]; [ reflexivity | ].
     apply bind_mon; [ apply popA_mon; auto | intros ? ? []; [ reflexivity | ] ].
     destruct x1, y0.
-    apply ret_mon. repeat (constructor + apply H).
+    apply bind_mon; [ apply force_mon, H | intros ].
+    apply ret_mon. constructor; [ assumption | constructor ].
 Qed.
 
-#[global] Instance ImplApprox_Queue : ImplApprox Op (Queue a) TQueueA.
+#[global] Instance ImplApprox_Queue : ImplApprox Op (Queue a) QAa.
 Proof.
   econstructor; try typeclasses eauto.
 Defined.
 
 (* "debt" in BankersQueue *)
-Definition potential : TQueueA -> nat := fun Tq =>
-  match Tq with
-  | Undefined => 0
-  | Thunk qA => 2 * sizeX 0 (frontA qA) - 2 * nbackA qA
-  end.
+Definition potential : QAa -> nat := fun qA =>
+  2 * sizeX 0 (frontA qA) - 2 * nbackA qA.
 
-Lemma potential_lub_QueueA : forall qA qA' : TQueueA, cobounded qA qA' -> potential (lub qA qA') <= potential qA + potential qA'.
+Lemma potential_lub_QueueA : forall qA qA' : QAa, cobounded qA qA' -> potential (lub qA qA') <= potential qA + potential qA'.
 Proof.
-  unfold TQueueA. apply @LubDebt_T, @LubDebt_QueueA.
+  apply @LubDebt_QueueA.
 Qed.
 
-#[global] Instance HasAmortizedCost_Queue : HasAmortizedCost Op (Queue a) TQueueA.
+#[global] Instance HasAmortizedCost_Queue : HasAmortizedCost Op (Queue a) QAa.
 Proof.
   apply Build_HasAmortizedCost with (potential := potential).
   - exact @potential_lub_QueueA.
