src/FingerTreeInterface.v
@@ -1,0 +1,122 @@
+(* Instantiate Interfaces with FingerTreeM *)
+
+(* Note: finger trees use laziness: [consA] and [snocA] are recursive,
+   so one could try to apply them repeatedly to a "dangerous" tree
+   to take O(log n) time every time instead of O(1).
+   But the recursive calls are to be forced (and amortized) by future
+   operations. *)
+From Coq Require Import List RelationClasses.
+From Clairvoyance Require Import
+  Core Approx ApproxM List Misc Cost Interfaces.
+From Clairvoyance Require FingerTree FingerTreeM.
+
+Import ListNotations.
+
+Set Primitive Projections.
+Set Implicit Arguments.
+Set Contextual Implicit.
+Set Maximal Implicit Insertion.
+
+Definition a := nat.
+
+(** Operations symbols *)
+Inductive Op : Type :=
+| Empty
+| Cons (x : a)
+| Snoc (x : a)
+| Head
+| Tail
+| Append
+.
+
+(* Pure reference implementation [eval_op_Seq] and cost specification [CostSpec_Seq] *)
+Section Seq.
+Import FingerTree.
+
+Definition Seq := FingerTree.Seq.
+
+Definition eval_op_Seq (o : Op) (vs : list (Seq a)) : list (Seq a) :=
+  match o, vs with
+  | Empty, _ => [Nil]
+  | Cons x, q :: _ => [cons x q]
+  | Snoc x, q :: _ => [snoc q x]
+  | Head, q :: _ => []  (* Doesn't create a new FT *)
+  | Tail, q :: _ => [tail q]
+  | Append, q :: q' :: _ => [append q q']
+  | _, _ => []
+  end.
+
+(* TODO: splitAt, as an example of operation with two outputs *)
+
+#[global] Instance PureImpl_Seq : PureImpl Op (Seq a) := eval_op_Seq.
+
+#[global] Instance CostSpec_Seq : CostSpec Op (Seq a) :=
+  fun o vs =>
+    match o, vs with
+    | (Empty | Cons _ | Snoc _ | Head | Tail), _ => 1
+    | Append, q :: q' :: _ => max (depth q) (depth q')
+    | _, _ => 0
+    end.
+
+End Seq.
+
+(* Clairvoyant translation *)
+Section SeqA.
+Import FingerTreeM.
+
+Definition SeqA' := SeqA a.
+
+Definition exec_op_SeqA (o : Op) (vs : list SeqA') : M (list SeqA') :=
+  match o, vs with
+  | Empty, _ => ret [Nil]
+  | Cons x, q :: _ => let! q := consA (Thunk x) (Thunk q) in ret [q]
+  | Snoc x, q :: _ => let! q := snocA (Thunk q) (Thunk x) in ret [q]
+  | Head, q :: _ => let! _ := headA (Thunk q) in ret []  (* Doesn't create a new FT *)
+  | Tail, q :: _ => let! q := tailA (Thunk q) in ret [q]
+  | Append, q :: q' :: _ => let! q := appendA (Thunk q) (Thunk q') in ret [q]
+  | _, _ => ret []
+  end.
+
+#[global] Instance CvImpl_SeqA : CvImpl Op SeqA' := exec_op_SeqA.
+
+(** ** [ImplApprox_Seq]: Order structure of [SeqA] *)
+
+#[global] Instance Exact_Seq : Exact (Seq a) (SeqA a).
+Admitted.
+
+#[global] Instance LessDefined_SeqA : LessDefined (SeqA a).
+Admitted.
+
+#[global] Instance PreOrder_less_defined_SeqA : PreOrder (less_defined (a := SeqA a)).
+Admitted.
+
+#[global] Instance Lub_SeqA : Lub (SeqA a). Admitted.
+#[global] Instance LubLaw_SeqA : LubLaw (SeqA a). Admitted.
+
+#[local] Instance exec_op_mon (o : Op) :
+  Morphisms.Proper (Morphisms.respectful less_defined less_defined)
+    (exec_op (op := Op) (valueA := SeqA') o).
+Proof.
+Admitted.
+
+#[global] Instance ImplApprox_Seq : ImplApprox Op (Seq a) SeqA'.
+Proof.
+  econstructor; try typeclasses eauto.
+Defined.
+
+(** * Main theorem: HasAmortizedCost_Seq *)
+
+(* "debt" in BankersSeq *)
+Definition potential : SeqA' -> nat := fun t =>
+  0 (* TODO *).
+
+Lemma potential_lub_SeqA : forall qA qA' : SeqA', cobounded qA qA' -> potential (lub qA qA') <= potential qA + potential qA'.
+Proof.
+Admitted.
+
+#[global] Instance HasAmortizedCost_Seq : HasAmortizedCost Op (Seq a) SeqA'.
+Proof.
+  apply Build_HasAmortizedCost with (potential := potential).
+  - exact @potential_lub_SeqA.
+  - admit.
+Admitted.
